feat: change Pointer.Reduction to have an initial pointer
This makes some reasonings way easier since buildTree only uses the
first pointer, so they rest doesn't have to uphold Invariants.
The reasoning when merging gets very messy.

Earley/Recognizer.lean
@@ -79,7 +79,7 @@ inductive Pointer where
   /-- .scan: origin index for previous bin. -/
   | predecessor (i : Nat) : Pointer
   /-- .complete: nonempty list of possible reduction pointers -/
-  | reduction (ps : List ReductionPointer) : Pointer
+  | reduction (p : ReductionPointer) (ps : List ReductionPointer) : Pointer
 deriving BEq, Repr
 
 /--
@@ -126,16 +126,8 @@ public def isWellFormedBinItems (G : ContextFreeGrammarList T N) (w : List T) (k
   (items bin).Nodup ∧
     ∀ x ∈ bin, isWellFormed G.rules (w.map Symbol.terminal) x.item ∧ x.item.endIdx = k
 
-@[grind]
-public def isNonEmptyPointer (pointer : Pointer) : Prop :=
-  match pointer with
-  | .null | .predecessor _ => True
-  | .reduction ps => ps ≠ []
-
 /--
 The pointers of an EarleyBin are well-formed, if
-- TODO
-
 TODO: rethink naming scheme since it has to be split weirdly in two
       Since the pointers require access to previous bins, it's a bit inconvenient to merge.
       I could make isWellFormedBinPointers reason about the index and simply merge?
@@ -150,7 +142,7 @@ public def isWellFormedPointer (w : List T) (bins : EarleyBins T N (w.length + 1
   match pointer with
   | .null => True
   | .predecessor i => k ≠ 0 ∧ k - 1 ≤ w.length ∧ ((h : k - 1 ≤ w.length) → i < bins[k-1].length)
-  | .reduction ps => k ≤ w.length ∧ ps ≠ [] ∧ ∀ p ∈ ps, p.endIdxA ≤ w.length ∧
+  | .reduction p ps => k ≤ w.length ∧ p.endIdxA ≤ w.length ∧
       ((h : p.endIdxA ≤ w.length) → p.i < bins[p.endIdxA].length) ∧
       ((h : k ≤ w.length) → p.j < bins[k].length)
 
@@ -159,11 +151,16 @@ public def isWellFormedBinPointers (w : List T) (bins : EarleyBins T N (w.length
     (bin : List (BinItem T N)) (k : Nat) : Prop :=
   ∀ x ∈ bin, isWellFormedPointer w bins x.pointer k
 
+/--
+Interestingly enough, we only reason about the first pointer
+since it is the only one used for buildTree anyway.
+There are problematic details when merging reduction pointers.
+-/
 @[grind]
 public def isSoundPointer (pointer : Pointer) (k j : Nat) : Prop :=
   match pointer with
   | .null | .predecessor _ => True
-  | .reduction ps => ∀ p ∈ ps, (p.endIdxA < k ∨ (p.endIdxA = k ∧ p.i < j)) ∧ p.j < j
+  | .reduction p _ => (p.endIdxA < k ∨ (p.endIdxA = k ∧ p.i < j)) ∧ p.j < j
 
 /--
 EarleyBins are well-formed, if all of its bins are well-formed.
@@ -228,7 +225,7 @@ def completeList (y : EarleyItem T N) (n : Nat) (bins : EarleyBins T N n) (h : y
     (fun x => nextSymbol x.item == some (Symbol.nonterminal y.rule.input))
   -- Matchings mapped onto a new item with the index recorded within the reduction pointer
   xMatches.map (fun ⟨x,i⟩ =>
-    ⟨incItem x.item y.endIdx, Pointer.reduction [⟨y.startIdx,i,j⟩]⟩)
+    ⟨incItem x.item y.endIdx, Pointer.reduction ⟨y.startIdx,i,j⟩ []⟩)
 
 /--
 Returns the list appended with an element, if it is not already part of the list,
@@ -239,10 +236,10 @@ Predecessor pointers are unique, so duplicate items can be safely discarded
 def updateBinAux : List (BinItem T N) → BinItem T N → List (BinItem T N)
   | [], y => [y]
   | x::xs, y => match (x,y) with
-    | (⟨xItem, Pointer.reduction xP⟩,⟨yItem, Pointer.reduction yP⟩) =>
+    | (⟨xItem, Pointer.reduction xp xP⟩,⟨yItem, Pointer.reduction yp yP⟩) =>
       -- Merge any reduction pointers if the items match
       if xItem == yItem then
-        ⟨xItem, Pointer.reduction (xP.append yP)⟩::xs
+        ⟨xItem, Pointer.reduction xp (yp::xP.append yP)⟩::xs
       else
         -- Search further, if no match
         x::(updateBinAux xs y)
@@ -411,11 +408,11 @@ lemma updateBinAux_of_Red_of_neqItem (xs : List (BinItem T N)) (y : BinItem T N)
     grind [updateBinAux_of_Red_of_neqItemAux]
 
 theorem updateBinAux_of_updRed (xs xs' : List (BinItem T N)) (y : BinItem T N) (i : Nat)
-    (hNoDup : (items xs).Nodup) {xP yP : List ReductionPointer}
-    (hi : i < xs.length) (hx : xs[i].pointer = Pointer.reduction xP) (heq : y.item = xs[i].item)
-    (hy : y.pointer = .reduction yP) (hxs' : xs' = updateBinAux xs y) :
+    (hNoDup : (items xs).Nodup) {xp yp : ReductionPointer} {xP yP : List ReductionPointer}
+    (hi : i < xs.length) (hx : xs[i].pointer = Pointer.reduction xp xP) (heq : y.item = xs[i].item)
+    (hy : y.pointer = .reduction yp yP) (hxs' : xs' = updateBinAux xs y) :
     xs'.length = xs.length ∧ ((hlen : xs'.length = xs.length) →
-    xs'[i].pointer = .reduction (xP.append yP) ∧
+    xs'[i].pointer = .reduction xp (yp::xP.append yP) ∧
     (∀ j, (hj : j < xs'.length ∧ i ≠ j) → xs'[j] = xs[j]'(by lia))) := by
   induction xs generalizing i y xs' with
   | nil => grind
@@ -427,14 +424,14 @@ theorem updateBinAux_of_updRed (xs xs' : List (BinItem T N)) (y : BinItem T N) (
     · if h : x.item = y.item then
         clear ih
         simp only [updateBinAux, beq_iff_eq, List.append_eq]
-        have hxP : x.pointer = Pointer.reduction xP := by grind
-        have hx2 : x = ⟨x.item, Pointer.reduction xP⟩ := by rw [← hxP]
-        have hy2 : y = ⟨x.item, Pointer.reduction yP⟩ := by rw [← hy]; rw [h]
+        have hxP : x.pointer = Pointer.reduction xp xP := by grind
+        have hx2 : x = ⟨x.item, Pointer.reduction xp xP⟩ := by rw [← hxP]
+        have hy2 : y = ⟨x.item, Pointer.reduction yp yP⟩ := by rw [← hy]; rw [h]
         grind
       else
         have hi : i - 1 < xs.length := by grind
         specialize ih (updateBinAux xs y) y (i-1) (by grind [List.Nodup.of_cons]) hi
-        have xs1 : xs[i - 1].pointer = Pointer.reduction xP := by grind
+        have xs1 : xs[i - 1].pointer = Pointer.reduction xp xP := by grind
         have h2 : y.item = xs[i - 1].item := by grind
         specialize ih xs1 h2 hy (by simp)
         have ⟨h3, _⟩ := ih.right ih.left
@@ -444,15 +441,16 @@ theorem updateBinAux_of_updRed (xs xs' : List (BinItem T N)) (y : BinItem T N) (
       grind
 
 lemma updateBinAux_of_Red_of_eqItem (xs : List (BinItem T N)) (y : BinItem T N) (i j : Nat)
-    (hNoDup : (items xs).Nodup) {yP : List ReductionPointer} (hy : y.pointer = .reduction yP)
-    (hi : i < xs.length) (hx : xs[i].pointer = .null ∨ xs[i].pointer = .predecessor j)
-    (heq : y.item = xs[i].item) : updateBinAux xs y = xs := by
+    (hNoDup : (items xs).Nodup) {yp : ReductionPointer} {yP : List ReductionPointer}
+    (hy : y.pointer = .reduction yp yP) (hi : i < xs.length)
+    (hx : xs[i].pointer = .null ∨ xs[i].pointer = .predecessor j) (heq : y.item = xs[i].item) :
+    updateBinAux xs y = xs := by
   induction xs generalizing i with
   | nil => grind
   | cons x xs ih => grind
 
 lemma wfBinPointers_of_updateBinAux (w : List T) {k : Nat} (bins : EarleyBins T N (w.length + 1))
-    (hk : k < w.length + 1) (xs : List (BinItem T N)) (hwfbin : isWellFormedBinPointers w bins xs k)
+    (xs : List (BinItem T N)) (hwfbin : isWellFormedBinPointers w bins xs k)
     (y : BinItem T N) (hwfy : isWellFormedPointer w bins y.pointer k) :
     isWellFormedBinPointers w bins (updateBinAux xs y) k := by
   induction xs with
@@ -462,15 +460,12 @@ lemma wfBinPointers_of_updateBinAux (w : List T) {k : Nat} (bins : EarleyBins T 
     simp only [isWellFormedBinPointers] at ih
     split
     · split
-      · rename_i xP _ yP heq h
+      · rename_i xp xP _ yp yP heq h
         -- FIXME: this screams missing deconstruction?
-        have hxP : x.pointer = Pointer.reduction xP := by grind
-        have hx2 : x = ⟨x.item, Pointer.reduction xP⟩ := by grind
-        have hy2 : y = ⟨x.item, Pointer.reduction yP⟩ := by grind
-        simp only [isWellFormedPointer, hy2, ne_eq] at hwfy
-        have : xP ++ yP ≠ [] := by
-          have : yP ≠ [] := by grind
-          simp [this]
+        have hxP : x.pointer = Pointer.reduction xp xP := by grind
+        have hx2 : x = ⟨x.item, Pointer.reduction xp xP⟩ := by grind
+        have hy2 : y = ⟨x.item, Pointer.reduction yp yP⟩ := by grind
+        simp only [isWellFormedPointer, hy2] at hwfy
         grind
       · grind
     · split <;> grind
@@ -484,20 +479,19 @@ lemma wfBinItems_of_updateBin (G : ContextFreeGrammarList T N) (w : List T) {k :
   | cons y ys ih => grind [wfBinItems_of_updateBinAux, noDup_of_updateBin]
 
 lemma wfBinPointers_of_updateBin (w : List T) {k : Nat} (bins : EarleyBins T N (w.length + 1))
-    (hk : k < w.length + 1) (xs : List (BinItem T N)) (hwfbin : isWellFormedBinPointers w bins xs k)
+    (xs : List (BinItem T N)) (hwfbin : isWellFormedBinPointers w bins xs k)
     (ys : List (BinItem T N)) (hwfy : ∀ y ∈ ys, isWellFormedPointer w bins y.pointer k) :
     isWellFormedBinPointers w bins (updateBin xs ys) k := by
   induction ys generalizing xs with
   | nil => grind
   | cons y ys ih =>
-    have hwfAux := wfBinPointers_of_updateBinAux w bins hk xs hwfbin y (by grind)
+    have hwfAux := wfBinPointers_of_updateBinAux w bins xs hwfbin y (by grind)
     grind
 
-lemma soundPointers_of_updateBinAux (G : ContextFreeGrammarList T N) (w : List T) {k : Nat}
-    (bins : EarleyBins T N (w.length + 1)) (hbins : ∀ k, (hk : k ≤ w.length) →
-     (items bins[k]).Nodup ∧ ∀ j, (hj : j < bins[k].length) → isSoundPointer bins[k][j].pointer k j)
-    (y : BinItem T N) (hnEmpty : isNonEmptyPointer y.pointer) (hk : k < w.length + 1)
-    (hwf : isSoundPointer y.pointer k bins[k].length) :
+lemma soundPointers_of_updateBinAux (w : List T) {k : Nat} (bins : EarleyBins T N (w.length + 1))
+    (hbins : ∀ k, (hk : k ≤ w.length) → (items bins[k]).Nodup ∧ ∀ j, (hj : j < bins[k].length)
+      → isSoundPointer bins[k][j].pointer k j)
+    (y : BinItem T N) (hk : k < w.length + 1) (hwf : isSoundPointer y.pointer k bins[k].length) :
     ∀ j, (hj : j < (updateBinAux bins[k] y).length) →
     isSoundPointer (updateBinAux bins[k] y)[j].pointer k j := by
   have : y.item ∉ items bins[k] ∨
@@ -512,7 +506,7 @@ lemma soundPointers_of_updateBinAux (G : ContextFreeGrammarList T N) (w : List T
   · simp only [not_exists, not_or] at hnex
     match hy : y.pointer with
     | .null | .predecessor i => grind [hnex 0]
-    | .reduction yPs =>
+    | .reduction yp yP =>
       have := List.getElem_of_mem hmem
       rcases this with ⟨j', hjI', heq⟩
       have hj' : j' < bins[k].length := by grind
@@ -532,37 +526,19 @@ lemma soundPointers_of_updateBinAux (G : ContextFreeGrammarList T N) (w : List T
           simp [heq]
         have := updateBinAux_of_Red_of_eqItem bins[k] y j' i this hy (by grind) (by simp [hb]) heq'
         grind
-      | .reduction bPs =>
+      | .reduction bp bP =>
         have hnDup := (hbins k (by grind)).left
         have : y.item = bins[k][j'].item := by grind
         have hupdRed := updateBinAux_of_updRed bins[k] (updateBinAux bins[k] y) y j' hnDup hj'
             hb this hy (by simp)
-        intro j hj
-        simp only [isSoundPointer]
-        rcases hPs : (updateBinAux bins[k] y)[j].pointer with _ | _ | ps <;> simp only
-        intro p hp
-        if heq : j = j' then
-          constructor
-          · sorry
-          · have : (updateBinAux bins[k] y)[j'].pointer = .reduction (bPs ++ yPs) := by
-              simp [hupdRed]
-            have : ps = bPs ++ yPs := by grind
-            have : ∀ p ∈ bPs, p.j < j := by grind
-            have : ∀ p ∈ yPs, p.j < j := by
-              have hwf := hwf
-              simp [isSoundPointer, hy] at hwf
-              sorry
-            grind
-        else
-          grind
+        grind
 
 -- I cannot really simplify the goal and make the proof easier for me
 -- since any item of ys can get merged into the bins and thus the `< j` would get problematic.
-lemma soundPointers_of_updateBin (G : ContextFreeGrammarList T N) (w : List T) (k : Nat)
-    (bins : EarleyBins T N (w.length + 1)) (hbins : ∀ k, (hk : k ≤ w.length) →
-     (items bins[k]).Nodup ∧ ∀ j, (hj : j < bins[k].length) → isSoundPointer bins[k][j].pointer k j)
+lemma soundPointers_of_updateBin (w : List T) (k : Nat) (bins : EarleyBins T N (w.length + 1))
+    (hbins : ∀ k, (hk : k ≤ w.length) → (items bins[k]).Nodup ∧ ∀ j, (hj : j < bins[k].length)
+      → isSoundPointer bins[k][j].pointer k j)
     (ys : List (BinItem T N)) (hk : k < w.length + 1)
-    (hnEmpty : ∀ y ∈ ys, isNonEmptyPointer y.pointer)
     (hwf : ∀ y ∈ ys, isSoundPointer y.pointer k bins[k].length) :
     ∀ j, (hj : j < (updateBin bins[k] ys).length) →
     isSoundPointer (updateBin bins[k] ys)[j].pointer k j := by
@@ -571,7 +547,7 @@ lemma soundPointers_of_updateBin (G : ContextFreeGrammarList T N) (w : List T) (
   | cons y ys ih =>
     intro j hj
     let bins' := Vector.set bins k (updateBinAux bins[k] y) hk
-    have hSaux := soundPointers_of_updateBinAux G w bins hbins y (by grind) hk (by grind)
+    have hSaux := soundPointers_of_updateBinAux w bins hbins y hk (by grind)
     have : ∀ y ∈ ys, isSoundPointer y.pointer k bins'[k].length := by
       clear ih
       simp only [isSoundPointer]
@@ -599,19 +575,14 @@ lemma wfBins_of_updateBin (G : ContextFreeGrammarList T N) (w : List T) {k : Nat
     · have ⟨h1,h2,h3⟩ := hwf k (by lia)
       simp only [heq]
       have hwfb : isWellFormedBinPointers w bins (updateBins bins k ys hk)[k] k := by
-        have := wfBinPointers_of_updateBin w bins (by lia) bins[k] h2 ys (by grind)
+        have := wfBinPointers_of_updateBin w bins bins[k] h2 ys (by grind)
         grind
       have : ∀ (i : ℕ) (hi : i ≤ w.length), bins[i].length
           ≤ (updateBins bins k ys hk)[i].length := by grind [lengthNth_le_lengthUpdateBinNth]
       have := wfBinPointers_of_updatedBins w bins (updateBins bins k ys hk) hk this hwfb
       grind
     · intro j hj
-      have : ∀ y ∈ ys, isNonEmptyPointer y.pointer := by
-        intro y hmemy
-        specialize hwfPy y hmemy
-        simp only [isWellFormedPointer, ne_eq, tsub_le_iff_right] at hwfPy
-        grind
-      have := soundPointers_of_updateBin G w k bins (by grind) ys
+      have := soundPointers_of_updateBin w k bins (by grind) ys
       grind
   else
     refine ⟨by grind, ?_⟩
@@ -725,9 +696,9 @@ lemma wfPointers_of_completeList {G : ContextFreeGrammarList T N} {w : List T} (
   simp only [isWellFormedPointer, tsub_le_iff_right]
   -- z is the original item, which will be completed
   rcases hmemx with ⟨z,zIdx,⟨hmemz,hx⟩⟩
-  have xP : x.pointer = Pointer.reduction [{ endIdxA := y.startIdx, i := zIdx, j := j }] := by grind
-  simp only [xP, List.mem_cons, List.not_mem_nil, or_false, forall_eq]
-  refine ⟨by lia, by simp, by grind, ?_, by grind⟩
+  have xP : x.pointer = Pointer.reduction ⟨y.startIdx, zIdx, j⟩ [] := by grind
+  simp only [xP]
+  refine ⟨by lia, by grind, ?_, by grind⟩
   intro hbounds
   have := filterWithIdx_le_length bins[y.startIdx]
     (fun x => x.item.nextSymbol == some (Symbol.nonterminal y.rule.input)) zIdx (by grind)
@@ -748,8 +719,8 @@ lemma soundPointers_of_completeList (G : ContextFreeGrammarList T N) {w : List T
   let filteredOriginBin := filterWithIdx originBin P
   -- z is the original item, which will be completed
   rcases hmemx with ⟨z,zIdx,⟨hmemz,hx⟩⟩
-  have xP : x.pointer = Pointer.reduction [{ endIdxA := y.startIdx, i := zIdx, j := j }] := by grind
-  simp only [xP, List.mem_cons, List.not_mem_nil, or_false, forall_eq]
+  have xP : x.pointer = Pointer.reduction ⟨y.startIdx, zIdx, j⟩ [] := by grind
+  simp only [xP]
   refine ⟨?_, by grind⟩
   simp only [isWellFormedBins, Order.lt_add_one_iff] at hbins
   specialize hbins k (by grind)
